Week5/Solved/ASD1/prob5.dfy
@@ -1,38 +1,20 @@
 // Problema 5
 
-function pow(base: int, exp: nat): int {
-    if exp == 0 then 1 else base * pow(base, exp - 1)
+method inversare(n: nat) returns (m: nat)
+  requires n >= 0
+  ensures m == Reverse(n)
+{
+  m := reverseHelper(n, 0);
 }
 
-// method inversare(n: nat) returns (m: nat)
-//   requires n == sum(set i: int | 0 <= i <= k :: c[i] * pow(10, i)) 
-//   ensures m == sum(set i: int | 0 <= i <= k :: c[i] * pow(10, k-i)) 
-// {
-//   m := 0;
-//   var p := 0;
-//   while n > 0
-//     invariant m == sum(set i: int | 0 <= i < p :: c[i] * pow(10, p-1-i))
-//     invariant n == sum(set i: int | p <= i <= k :: c[i] * pow(10, i-p)) 
-//     decreases n 
-//   {
-//     p := p + 1;
-//     m := m * 10 + n % 10;
-//     n := n / 10;
-//   }
-// }
-
-method inversare(n: int) returns (inversat: int)
-    requires n >= 0
+function Reverse(n: nat): nat
 {
-    inversat := 0;
-    var num := n;
-    var p := 0;
+  if n == 0 then 0 else reverseHelper(n, 0)
+}
 
-    while num > 0
-        decreases num
-    {
-        p := p + 1;
-        inversat := inversat * 10 + num % 10;
-        num := num / 10;
-    }
+function reverseHelper(n: nat, acc: nat): nat
+  decreases n
+{
+  if n == 0 then acc
+  else reverseHelper(n / 10, acc * 10 + n % 10)
 }
