Week5/Solved/ASD1/prob7.dfy
@@ -1,20 +1,20 @@
 // Problema 7
 
 method inversare_sir(x: array<int>) returns (y: array<int>)
-    requires forall i :: 1 <= i <= x.Length ==> x[i] == y[i]
-    ensures forall i :: 1 <= i <= x.Length ==> x[i] == y[x.Length + 1 - i]
+  requires 1 <= x.Length
+  ensures y.Length == x.Length
+  ensures forall i :: 0 <= i < x.Length ==> y[i] == x[x.Length - 1 - i]
 {
-    y := x;
-    var i := 0;
-    while i < (x.Length + 1) / 2
-        invariant 1 <= i <= (x.Length + 1) / 2
-        invariant forall j :: 1 <= j < i ==> x[j] == y[x.Length + 1 - j]
-        invariant forall j :: x.Length + 1 - i <= j <= x.Length ==> x[j] == y[x.Length + 1 - j]
-    {   
-        i := i + 1;
-        var temp := y[i];
-        y[i] := y[x.Length + 1 - i];
-        y[x.Length + 1 - i] := temp;
-        
-    }
+  var n := x.Length;
+  y := new int[n];
+  var i := 0;
+
+  while i < n
+    invariant 0 <= i <= n
+    invariant forall j :: 0 <= j < i ==> y[j] == x[n - 1 - j]
+    invariant y.Length == x.Length
+  {
+    y[i] := x[n - 1 - i];
+    i := i + 1;
+  }
 }
